Define forwardFD, linesFD, STD_OstreamFD
And maybe some other constants. Prove various properties about them.
Update proofs that were using bumpFD (and bumpLineFD, bumpAllFD) to use
the forward variants instead, since these formally ignore numchars -- I
realised that numchars should _only_ be used for the read system call.
At the STDIO level it is better to leave it untouched.

STD_OstreamFD is my workaround for the fact that the datatypes seem to
allow reading from stdout. The condition ¬STD_OstreamFD fs fd states
that fd is not a file descriptor for stdout or stderr, so reading from
it won't mess with outputting.

basis/fsFFIProofScript.sml
@@ -295,6 +295,7 @@ val ffi_close_length = Q.store_thm("ffi_close_length",
   \\ Cases_on`closeFD (w2n (HD bytes)) fs` \\ fs[] \\ rw[]
   \\ pairarg_tac \\ fs[] \\ rw[]);
 
+(* TODO: move *)
 (* insert a string (l1) at specified index (n) in a list (l2) *)
 val insert_atI_def = Define`
   insert_atI l1 n l2 =
@@ -330,14 +331,14 @@ val insert_atI_app = Q.store_thm("insert_atI_app",
 val insert_atI_end = Q.store_thm("insert_atI_end",
   `insert_atI l1 (LENGTH l2) l2 = l2 ++ l1`,
   simp[insert_atI_def,DROP_LENGTH_TOO_LONG]);
+(* -- *)
 
-(* TODO: used? *)
-val bumpAllFD_def = Define`
-  bumpAllFD fd fs =
+val fastForwardFD_def = Define`
+  fastForwardFD fs fd =
     the fs (do
       (fnm,off) <- ALOOKUP fs.infds fd;
       content <- ALOOKUP fs.files fnm;
-      SOME (fs with infds updated_by ALIST_FUPDKEY fd (I ## (MAX (LENGTH content))))
+      SOME (fs with infds updated_by ALIST_FUPDKEY fd (I ## MAX (LENGTH content)))
     od)`;
 
 val LUPDATE_insert_commute = Q.store_thm(
@@ -355,26 +356,29 @@ val getNullTermStr_insert_atI = Q.store_thm(
   simp[getNullTermStr_def, insert_atI_def, findi_APPEND, NOT_MEM_findi,
        findi_def, TAKE_APPEND])
 
-val validFD_bumpAllFD = Q.store_thm("validFD_bumpAllFD[simp]",
-  `validFD fd (bumpAllFD fd fs) = validFD fd fs`,
-  rw[validFD_def,bumpAllFD_def]
+val validFD_fastForwardFD = Q.store_thm("validFD_fastForwardFD[simp]",
+  `validFD fd (fastForwardFD fs fd) = validFD fd fs`,
+  rw[validFD_def,fastForwardFD_def,bumpFD_def]
   \\ Cases_on`ALOOKUP fs.infds fd` \\ fs[libTheory.the_def]
   \\ pairarg_tac \\ fs[]
-  \\ Cases_on`ALOOKUP fs.files fnm` \\ fs[libTheory.the_def]);
+  \\ Cases_on`ALOOKUP fs.files fnm` \\ fs[libTheory.the_def]
+  \\ rw[OPTION_GUARD_COND,libTheory.the_def]);
 
-val bumpAllFD_files = Q.store_thm("bumpAllFD_files[simp]",
-  `(bumpAllFD fd fs).files = fs.files`,
+val fastForwardFD_files = Q.store_thm("fastForwardFD_files[simp]",
+  `(fastForwardFD fs fd).files = fs.files`,
   EVAL_TAC
   \\ Cases_on`ALOOKUP fs.infds fd` \\ fs[libTheory.the_def]
   \\ pairarg_tac \\ fs[]
-  \\ Cases_on`ALOOKUP fs.files fnm` \\ fs[libTheory.the_def]);
+  \\ Cases_on`ALOOKUP fs.files fnm` \\ fs[libTheory.the_def]
+  \\ rw[OPTION_GUARD_COND,libTheory.the_def]);
 
-val A_DELKEY_bumpAllFD_elim = Q.store_thm("A_DELKEY_bumpAllFD_elim[simp]",
-  `A_DELKEY fd (bumpAllFD fd fs).infds = A_DELKEY fd fs.infds`,
-  rw[bumpAllFD_def]
+val A_DELKEY_fastForwardFD_elim = Q.store_thm("A_DELKEY_fastForwardFD_elim[simp]",
+  `A_DELKEY fd (fastForwardFD fs fd).infds = A_DELKEY fd fs.infds`,
+  rw[fastForwardFD_def,bumpFD_def]
   \\ Cases_on`ALOOKUP fs.infds fd` \\ fs[libTheory.the_def]
   \\ pairarg_tac \\ fs[]
-  \\ Cases_on`ALOOKUP fs.files fnm` \\ fs[libTheory.the_def]);
+  \\ Cases_on`ALOOKUP fs.files fnm` \\ fs[libTheory.the_def]
+  \\ rw[OPTION_GUARD_COND,libTheory.the_def]);
 
 val wfFS_fsupdate = Q.store_thm("wfFS_fsupdate",
     `! fs fd content pos k. wfFS fs ==> MEM fd (MAP FST fs.infds) ==>
@@ -477,11 +481,15 @@ val numchars_self = Q.store_thm("numchars_self",
  `!fs. fs = fs with numchars := fs.numchars`,
  cases_on`fs` >> fs[fsFFITheory.IO_fs_numchars_fupd]);
 
-val get_file_content_bumpFD = Q.store_thm("get_file_content_bumpFD",
- `!fs fd c pos n. get_file_content fs fd = SOME (c, pos) ==>
-  get_file_content (bumpFD fd fs n) fd = SOME(c, pos + n)`,
-    rw[bumpFD_def,get_file_content_def,ALIST_FUPDKEY_ALOOKUP] >>
-    pairarg_tac >> fs[]);
+val get_file_content_bumpFD = Q.store_thm("get_file_content_bumpFD[simp]",
+ `!fs fd c pos n.
+   get_file_content (bumpFD fd fs n) fd =
+   OPTION_MAP (I ## (+) n) (get_file_content fs fd)`,
+ rw[get_file_content_def,bumpFD_def,ALIST_FUPDKEY_ALOOKUP]
+ \\ CASE_TAC \\ fs[]
+ \\ pairarg_tac \\ fs[]
+ \\ pairarg_tac \\ fs[] \\ rw[]
+ \\ Cases_on`ALOOKUP fs.files fnm` \\ fs[]);
 
 (* TODO: in misc *)
 val ALIST_FUPDKEY_comm = Q.store_thm("ALIST_FUPDKEY_comm",
